Weidenbach_Book/IsaSAT/IsaSAT_LBD_LLVM.thy
@@ -1,0 +1,24 @@
+theory IsaSAT_LBD_LLVM
+  imports IsaSAT_LBD IsaSAT_Setup_LLVM
+begin
+
+sepref_register mark_lbd_from_clause_heur get_level_pol
+
+sepref_def mark_lbd_from_clause_heur_impl
+  is \<open>uncurry3 mark_lbd_from_clause_heur\<close>
+  :: \<open>trail_pol_fast_assn\<^sup>k *\<^sub>a arena_fast_assn\<^sup>k *\<^sub>a sint64_nat_assn\<^sup>k *\<^sub>a lbd_assn\<^sup>d \<rightarrow>\<^sub>a lbd_assn\<close>
+  unfolding mark_lbd_from_clause_heur_def nfoldli_upt_by_while
+  apply (rewrite at \<open>_ = \<hole>\<close> unat_const_fold[where 'a=32])
+  apply (annot_snat_const \<open>TYPE(64)\<close>) 
+  by sepref
+
+sepref_def calculate_LBD_heur_st_impl
+  is \<open>uncurry calculate_LBD_heur_st\<close>
+  :: \<open>isasat_bounded_assn\<^sup>d *\<^sub>a sint64_nat_assn\<^sup>k \<rightarrow>\<^sub>a isasat_bounded_assn\<close>
+  supply [[goals_limit=1]]
+  unfolding calculate_LBD_heur_st_def isasat_bounded_assn_def
+    fold_tuple_optimizations
+  apply (annot_unat_const \<open>TYPE(32)\<close>)
+  by sepref
+
+end
